compiler.v
@@ -5,21 +5,11 @@ From LF Require Import imports.
 From LF Require Import transforms.
 From LF Require Import python.
 
-Fixpoint convertValues (v : AbValue) : PyValue :=
-  match v with
-  | AbNat n => PyNat n
-  | AbBool b => PyBool b
-  end.
-
-Fixpoint numCompile (ae : AbNum) : PyNum :=
-  match ae with
-    | AbLit l => PyLit l
-    | AbId n => PyId n
-  end.
-
 Fixpoint numExprCompile (ae : AbNumExpr) : PyNumExpr :=
   match ae with
-    | AbNum2 n => PyNum2 (numCompile n)
+    | AbNatLit l => PyNatLit l
+    | AbIdNat n => PyIdNat n
+    | AbVectorValue s n => PyArrayValue s n
     | AbAdd a1 a2 => PyAdd (numExprCompile a1) (numExprCompile a2)
     | AbSub a1 a2 => PySub (numExprCompile a1) (numExprCompile a2)
     | AbMulti a1 a2 => PyMulti (numExprCompile a1) (numExprCompile a2)
@@ -29,6 +19,7 @@ Fixpoint binExprCompile (b : AbBinExpr) : PyBinExpr :=
   match b with
   | BinTrue => PyBinTrue
   | BinFalse => PyBinFalse
+  | AbIdBool s => PyIdBool s
   | AbUnaryOp b => PyUnaryOp (binExprCompile b)
   | AbLe a1 a2 => PyLe (numExprCompile a1) (numExprCompile a2)
   | AbEq a1 a2 => PyEq (numExprCompile a1) (numExprCompile a2)
@@ -49,23 +40,19 @@ Fixpoint compile (ac : AbCommand) : PyCommand :=
   | AbSeq c1 c2 => PySeq (compile c1) (compile c2)
   end.
 
-Compute compile (AbTransform "x" (Ab_Num_Expr (AbNum2 (AbLit 3)))).
-
-Theorem numEquiv : forall ab st,
-    AbEvalNumVal st ab = PyEvalNumVal st (numCompile ab).
-Proof.
-  intros; induction ab; reflexivity.
-Qed.
+Compute compile (AbTransform "x" (Ab_Num_Expr (AbNatLit (pNat 3)))).
 
 Theorem numExprEquiv : forall ab st,
     AbEvalNum st ab = PyEvalNum st (numExprCompile ab).
 Proof.
   intros.
-  induction ab;
-    (* Handles cases for AbAdd, AbSub, AbMulti *)
-    try ( induction ab1; induction ab2; simpl in *; rewrite IHab1; rewrite IHab2; reflexivity ).
-  - (* AbNum2 -> PyNum2 *)
-    induction n; reflexivity.
+  induction ab; simpl;
+    (* Solves cases: AbIdNat -> PyIdNat, AbArrayValue -> PyArrayValue *)
+    try destruct (st s);
+    (* Solves cases: AbAdd -> PyAdd, AbSub -> PySub, AbMulti -> PyMulti *)
+    try (rewrite IHab1;  rewrite IHab2);
+    (* Solves cases: AbNatLit -> PyNatLit *)
+    try reflexivity.
 Qed.
 
 Theorem binExprEquiv : forall ab st,
@@ -86,7 +73,7 @@ Proof.
 Qed.
 
 Theorem exprEquiv : forall ab st,
-    convertValues (AbEval st ab) = PyEval st (exprCompile ab).
+    AbEval st ab = PyEval st (exprCompile ab).
 Proof.
   intros. induction ab; simpl in *; try rewrite numExprEquiv; try rewrite binExprEquiv; reflexivity.
 Qed.
@@ -100,15 +87,9 @@ Proof.
   - (* AbTransform -> PyAssign *)
     induction a.
     + (* Ab_Num_Expr -> Py_Num_Expr *)
-      induction a; intros.
-      (* AbNum2 -> PyNum2 *)
-      induction n; simpl in *; inversion H; inversion H0; subst; reflexivity.
-      * (* AbAdd -> PyAdd *)
-        inversion H.
-      * (* AbSub -> PySub *)
-        inversion H.
-      * (* AbMulti -> PyMulti *)
-        inversion H.
+      induction a; intros; try inversion H.
+      (* AbNumLit -> PyNumLit *)
+      induction n; simpl in *; inversion H0; subst; reflexivity.
     + (* Ab_Bin_Expr -> Py_Bin_Expr *)
       induction b; intros; inversion H.
   - (* AbSeq -> PySeq *)
@@ -118,5 +99,5 @@ Proof.
     rewrite IHa2 with (st := st') (st1 := st'1) (st2 := st'2).
     reflexivity.
     assumption.
-    rewrite IHa1 with (st := st) (st1 := st') (st2 := st'0); assumption.  
+    rewrite IHa1 with (st := st) (st1 := st') (st2 := st'0); assumption.
 Qed.
