imports.v
@@ -1,4 +1,4 @@
-(** * Transform Language *)
+(** * Imports and common features used throughout the program *)
 Set Warnings "-notation-overridden,-parsing".
 Require Import Coq.Bool.Bool.
 Require Import Coq.Init.Nat.
@@ -10,7 +10,15 @@ Import ListNotations.
 
 From LF Require Export Maps.
 
-Definition state := total_map nat.
+(* Values: These are shared values both programs execute to *)
+Inductive prog_value : Type :=
+  | pNull
+  | pNat (n : nat)
+  | pBool (b : bool)
+  | pList (v : list nat).
+
+(* Defining the map to hold the state of the program *)
+Definition state := total_map prog_value.
 
 Reserved Notation "c1 '/' st '\\' st'"
                   (at level 40, st at level 39).
@@ -23,4 +31,28 @@ Fixpoint leb (n m : nat) : bool :=
       | O => false
       | S m' => leb n' m'
       end
+  end.
+
+(* Method to get a value from a list *)
+Fixpoint getValueList (v: list nat) (n : nat) : prog_value :=
+  match v with
+    | nil => pNull
+    | cons h t => match n with
+               | 0 => pNat h
+               | S n' => getValueList t n'
+                 end
+  end.
+
+(* Method to unwrap a nat from a prog_value *)
+Definition pullOutNat (v : prog_value) : nat :=
+  match v with
+  | pNat n => n
+  | _ => 0
+  end.
+
+(* Method to unwrap a bool from a prog_value *)
+Definition pullOutBool (v : prog_value) : bool :=
+  match v with
+  | pBool b => b
+  | _ => false
   end.
